{
  "@context": {
    "xsd":    "http://www.w3.org/2001/XMLSchema#",
    "rdf":    "http://www.w3.org/1999/02/22-rdf-syntax-ns#",
    "rdfs":   "http://www.w3.org/2000/01/rdf-schema#",
    "schema": "https://schema.org/",

    "coremo": "https://clipcode.org/base/schema/coremo/"
  },
  "@graph": [
    {
      "@id": "coremo:InformationContainer",
      "@type": "rdfs:Class",
      "rdfs:comment": "A container of information.",
      "rdfs:label": "InformationContainer",
      "rdfs:subClassOf": { "@id": "schema:CreativeWork" }
    }, 
    {
      "@id": "coremo:KnowledgeGraph",
      "@type": "rdfs:Class",
      "rdfs:comment": "A knowledge graph (which acts as a data container for one or more related semantic models).",
      "rdfs:label": "KnowledgeGraph",
      "rdfs:subClassOf": { "@id": "coremo:InformationContainer" }
    },
    {
      "@id": "coremo:SemanticModel",
      "@type": "rdfs:Class",
      "rdfs:comment": "A semantic model.",
      "rdfs:label": "SemanticModel",
      "rdfs:subClassOf": { "@id": "coremo:InformationContainer" }
    },
    {
      "@id": "coremo:hasSemanticModel",
      "@type": "rdf:Property",
      "rdfs:comment": "A semantic model that is contained within a knowledge graph.",
      "rdfs:label": "hasSemanticModel",
      "schema:domainIncludes": { "@id": "coremo:KnowledgeGraph" },
      "schema:rangeIncludes":  { "@id": "coremo:SemanticModel" }
    },
    {
      "@id": "coremo:SemanticPool",
      "@type": "rdfs:Class",
      "rdfs:comment": "A pool of semantic resources that manages a somewhat self-contained representation of an area of interest.",
      "rdfs:label": "SemanticPool",
      "rdfs:subClassOf": { "@id": "coremo:InformationContainer" }      
    },
    {
      "@id": "coremo:SemanticRoot",
      "@type": "rdfs:Class",
      "rdfs:comment": "A resource that can act as a root (directly attached to a semantic pool)",
      "rdfs:label": "SemanticRoot",
      "rdfs:subClassOf": { "@id": "coremo:InformationContainer" }      
    }
  ]
}
